sepcomp/stack.v
@@ -1,39 +1,33 @@
 Require Import ssreflect ssrbool ssrnat ssrfun eqtype seq fintype finfun.
 Set Implicit Arguments.
 
-Module Stack.
-Definition t (T : Type) := seq T.
-End Stack.
-
-Module StackDefs. Section stackDefs.
+Module SeqStack. Section seqStack.
 Variable T : Type.
 
-Import Stack.
-
 Definition updStack (newStack : seq T) := newStack.
-Definition push (stack: Stack.t T) (t: T) := updStack [:: t & stack].
-Definition peek (stack: Stack.t T) : option T :=
+Definition push (stack: seq T) (t: T) := updStack [:: t & stack].
+Definition peek (stack: seq T) : option T :=
   if stack is [:: topT & rest] then Some topT else None.
-Definition pop  (stack: Stack.t T) : Stack.t T := behead stack.
-Definition empty : Stack.t T := [::].
+Definition pop  (stack: seq T) : seq T := behead stack.
+Definition empty : seq T := [::].
 
-Definition nonempty : pred (Stack.t T) := 
+Definition nonempty : pred (seq T) := 
   [pred s | if s is [::] then false else true].
 
-Lemma peek_nonempty (stack : Stack.t T) t : 
+Lemma peek_nonempty (stack : seq T) t : 
   peek stack = Some t -> nonempty stack.
 Proof. by rewrite/peek; case: stack. Qed.
 
-Lemma nonempty_nempty (stack: Stack.t T) : nonempty stack -> [::] = stack -> T.
+Lemma nonempty_nempty (stack: seq T) : nonempty stack -> [::] = stack -> T.
 Proof. by case: stack. Qed.
 
-Definition head (stack: Stack.t T) (pf: nonempty stack) : T :=
+Definition head (stack: seq T) (pf: nonempty stack) : T :=
   (match stack as s return (s = stack -> T) with 
     | nil => fun pf' => nonempty_nempty pf pf'
     | s :: stack' => fun pf' => s
   end) erefl.
 
-Lemma nonempty_peek (stack : Stack.t T) (pf : nonempty stack) : 
+Lemma nonempty_peek (stack : seq T) (pf : nonempty stack) : 
   peek stack = Some (head stack pf).
 Proof. by move: pf; case: stack=>// a l _. Qed.
 
@@ -42,25 +36,60 @@ Lemma peeksome_head stack t :
   forall pf : nonempty stack, head stack pf = t.
 Proof. by rewrite/head; case: stack=> //=; move=> ? ?; case. Qed.
 
-Lemma all_pop (stack : Stack.t T) p : all p stack -> all p (pop stack).
+Lemma all_pop (stack : seq T) p : all p stack -> all p (pop stack).
 Proof. by case: stack=>//= a l; move/andP=> [H1 H2]. Qed.
 
-End stackDefs. End StackDefs.
+End seqStack. 
 
-(** Export push, pop, empty, nonempty, push_pop, pop_nonempty *)
-
-Notation push      := StackDefs.push.
-Notation pop       := StackDefs.pop.
-Notation peek      := StackDefs.peek.
-Notation head      := StackDefs.head.
-Notation empty     := StackDefs.empty.
-Notation nonempty  := StackDefs.nonempty.
-Notation peek_nonempty := StackDefs.peek_nonempty.
-Notation all_pop   := StackDefs.all_pop.
-
-Arguments StackDefs.updStack {T} !_ /.
+Arguments empty / {T}.
 Arguments push {T} _ _ /.
 Arguments pop {T} !_ /.
 Arguments peek {T} !_ /.
+Arguments nonempty {T} !_ /.
 Arguments head {T} !_ _ /.
-Arguments empty / {T}.
+
+End SeqStack.
+
+Module STACK. 
+
+Record type (T : Type) : Type := 
+  { t : Type
+  ; empty: t 
+  ; push : t -> T -> t
+  ; pop  : t -> t
+  ; peek : t -> option T
+  ; nonempty : pred t
+  ; head : forall t, nonempty t -> T
+  ; all  : pred T -> t -> bool 
+  ; all_pop : forall t p, all p t -> all p (pop t) }.
+
+End STACK.
+
+Arguments STACK.empty {T t} /.
+Arguments STACK.push {T t} _ _ /.
+Arguments STACK.pop {T t} _ /.
+Arguments STACK.peek {T t} _ /.
+Arguments STACK.nonempty {T t} _ /.
+Arguments STACK.head {T t} _ _ /.
+
+Coercion STACK.t : STACK.type >-> Sortclass.
+
+Module Stack.
+
+Import SeqStack.
+
+Section Stack.
+
+Variable T : Type.
+
+Definition t : STACK.type T := 
+  @STACK.Build_type T (seq T) empty push pop peek nonempty head 
+  all (@all_pop T).
+
+End Stack.
+
+End Stack.
+
+Canonical Structure seq_stackTy T : STACK.type T := Stack.t T.
+
+
